progs64/verif_append2.v fix proof2

progs64/verif_append2.v
@@ -16,11 +16,12 @@ Lemma nonidentity_not_bot : forall sh, sepalg.nonidentity sh -> sh <> Share.bot.
 Proof.
    intros. unfold sepalg.nonidentity. unfold not. intros. apply H. rewrite H0. apply bot_identity.    
 Qed.
-Hint Resolve not_bot_nonidentity : core.
-Hint Resolve nonidentity_not_bot : core.
+#[export] Hint Resolve not_bot_nonidentity : core.
+#[export] Hint Resolve nonidentity_not_bot : core.
+
 Section Spec.
 
-Context `{!default_VSTGS Σ}.
+Context  `{!default_VSTGS Σ}.
 
 Fixpoint listrep (sh: share)
             (contents: list val) (x: val) : mpred :=
@@ -96,8 +97,7 @@ Definition Gprog : funspecs :=   ltac:(with_library prog [ append_spec ]).
 Hint Resolve listrep_local_facts : saturate_local.
 Hint Resolve listrep_valid_pointer : valid_pointer.
 
-Definition lseg (sh: share) (contents: list val) (x z: val) : mpred :=
-  ∀ cts2:list val, listrep sh cts2 z -∗ listrep sh (contents++cts2) x.
+Section Proof1.
 
 Lemma body_append: semax_body Vprog Gprog ⊤ f_append append_spec.
 Proof.
@@ -144,6 +144,7 @@ forward_if.
 + (* after the loop *)
    clear v s1' Heqs1.
    forward.
+   simpl. (* TODO this simpl wasn't needed. maybe store_tac_no_hint in forward1 is broken? *)
    forward.
    rewrite (proj1 H2 (eq_refl _)).
    Exists x.
@@ -151,17 +152,19 @@ forward_if.
    clear.
    entailer!!.
    unfold listrep at 3; fold listrep. Intros.
-   unfold listrep at 2; fold listrep. Exists y; cancel.
+   iIntros "[[[Ha Hb] Hc] Hd]".
+   iApply "Ha".
+   unfold listrep at -1; fold listrep. iExists y; iFrame.
 Qed.
 
 End Proof1.
 
-Module Proof2.
+Section Proof2.
 
 Definition lseg (sh: share) (contents: list val) (x z: val) : mpred :=
-  ALL cts2:list val, listrep sh cts2 z -* listrep sh (contents++cts2) x.
+  ∀ cts2:list val, listrep sh cts2 z -∗ listrep sh (contents++cts2) x.
 
-Lemma body_append: semax_body Vprog Gprog f_append append_spec.
+Lemma body_append2: semax_body Vprog Gprog ⊤ f_append append_spec.
 Proof.
 start_function.
 forward_if.
@@ -178,7 +181,7 @@ forward_if.
  remember (v::s1') as s1.
  forward.
  forward_while
-      (EX s1a: list val,  EX a: val, EX s1b: list val, EX t: val, EX u: val,
+      (∃ s1a: list val, ∃ a: val, ∃ s1b: list val, ∃ t: val, ∃ u: val,
             PROP (s1 = s1a ++ a :: s1b)
             LOCAL (temp _x x; temp _t t; temp _u u; temp _y y)
             SEP (lseg sh s1a x t;
@@ -187,7 +190,7 @@ forward_if.
                    listrep sh s2 y))%assert.
 + (* current assertion implies loop invariant *)
    Exists (@nil val) v s1' x u.  entailer!!.
-   unfold lseg. apply allp_right; intro. simpl. cancel_wand.
+   unfold lseg. iIntros. simpl. auto.
 + (* loop test is safe to execute *)
    entailer!!.
 + (* loop body preserves invariant *)
@@ -200,101 +203,97 @@ forward_if.
    rewrite !app_ass. simpl app.
    entailer!!.
    unfold lseg.
-   rewrite sepcon_comm.
+   rewrite bi.sep_comm.
    clear.
-   apply RAMIF_Q.trans'' with (cons a).
-   extensionality cts; simpl; rewrite app_ass; reflexivity.
-   apply allp_right; intro. apply wand_sepcon_adjoint.
-   unfold listrep at 2; fold listrep; Exists u0.  apply derives_refl.
+   iIntros "[H1 H2]".
+   iIntros (cts2) "H3".
+   iSpecialize ("H2" $! (a :: cts2)).
+   rewrite app_ass.
+   iApply ("H2").
+   unfold listrep at -1; fold listrep. iExists u0. iFrame.
  + (* after the loop *)
-   forward. forward.
+   forward. simpl. forward.
    Exists x. entailer!!.
    destruct H3 as [? _]. specialize (H3 (eq_refl _)). subst s1b.
    unfold listrep at 1.  Intros. autorewrite with norm.  rewrite H0. rewrite app_ass. simpl app.
    unfold lseg.
-   rewrite sepcon_assoc.
-   eapply derives_trans; [apply allp_sepcon1 | ]. apply allp_left with (a::s2).
-   rewrite sepcon_comm.
-   eapply derives_trans; [ | apply modus_ponens_wand].
-   apply sepcon_derives; [ | apply derives_refl].
-   unfold listrep at 2; fold listrep. Exists y; auto.
+   rewrite -bi.sep_assoc.
+   iIntros "(H1 & H2 & H3)".
+   iApply ("H1" $! (a :: s2)).
+   unfold listrep at 2; fold listrep. iExists y; iFrame.
 Qed.
 
 End Proof2.
 
-Module Proof3.  (*************** inductive lseg *******************)
+Section Proof3.  (*************** inductive lseg *******************)
 
+Reset lseg.
 Fixpoint lseg (sh: share)
             (contents: list val) (x z: val) : mpred :=
  match contents with
- | h::hs => !! (x<>z) && 
-              EX y:val,
-                data_at sh t_struct_list (h,y) x * lseg sh hs y z
- | nil => !! (x = z /\ is_pointer_or_null x) && emp
+ | h::hs => ⌜x<>z⌝ ∧ 
+              ∃ y:val,
+                data_at sh t_struct_list (h,y) x ∗ lseg sh hs y z
+ | nil => ⌜x = z /\ is_pointer_or_null x⌝ ∧ emp
  end.
 
 Arguments lseg sh contents x z : simpl never.
 
 Lemma lseg_local_facts:
   forall sh contents p q,
-     lseg sh contents p q |--
-     !! (is_pointer_or_null p /\ is_pointer_or_null q /\ (p=q <-> contents=nil)).
+     lseg sh contents p q ⊢
+     ⌜is_pointer_or_null p /\ is_pointer_or_null q /\ (p=q <-> contents=nil)⌝.
 Proof.
 intros.
-apply derives_trans with (lseg sh contents p q && !! (is_pointer_or_null p /\
-        is_pointer_or_null q /\ (p = q <-> contents = []))).
+apply derives_trans with (lseg sh contents p q ∧ ⌜is_pointer_or_null p /\
+        is_pointer_or_null q /\ (p = q <-> contents = [])⌝).
 2: entailer!.
 revert p; induction contents; intros; simpl; unfold lseg; fold lseg.
 entailer!.
 intuition.
 Intros y. Exists y.
 eapply derives_trans.
-apply sepcon_derives.
+apply bi.sep_mono.
 apply derives_refl.
 apply IHcontents.
 entailer!.
 intuition congruence.
 Qed.
 
-#[export] Hint Resolve lseg_local_facts : saturate_local.
-
 Lemma lseg_valid_pointer:
   forall sh contents p ,
    sepalg.nonidentity sh ->
-   lseg sh contents p nullval |-- valid_pointer p.
+   lseg sh contents p nullval ⊢ valid_pointer p.
 Proof.
  destruct contents; unfold lseg; fold lseg; intros. entailer!.
  Intros *.
  auto with valid_pointer.
 Qed.
 
-#[export] Hint Resolve lseg_valid_pointer : valid_pointer.
-
 Lemma lseg_eq: forall sh contents x,
-    lseg sh contents x x = !! (contents=nil /\ is_pointer_or_null x) && emp.
+    lseg sh contents x x ⊣⊢ ⌜contents=nil /\ is_pointer_or_null x⌝ ∧ emp.
 Proof.
 intros.
 destruct contents; unfold lseg; fold lseg.
-f_equal. f_equal. f_equal. apply prop_ext; intuition.
-apply pred_ext.
-Intros y. contradiction.
-Intros. discriminate.
+- apply and_mono_iff; auto. apply bi.pure_iff. intuition.
+- iSplit. 
+  + iIntros "[%H1 H2]". contradiction.
+  + iIntros "[%H1 H2]". destruct H1. discriminate.
 Qed.
 
 Lemma lseg_null: forall sh contents,
-    lseg sh contents nullval nullval = !! (contents=nil) && emp.
+    lseg sh contents nullval nullval ⊣⊢ ⌜contents=nil⌝ ∧ emp.
 Proof.
 intros.
  rewrite lseg_eq.
- apply pred_ext.
- entailer!.
- entailer!.
+ apply and_mono_iff; auto.
+ apply bi.pure_iff; intuition.
 Qed.
 
-Lemma lseg_cons: forall sh (v u x: val) s,
+Lemma lseg_cons: forall sh (v u x: val) (s: list val),
    readable_share sh ->
- data_at sh t_struct_list (v, u) x * lseg sh s u nullval
- |-- lseg sh [v] x u * lseg sh s u nullval.
+ data_at sh t_struct_list (v, u) x ∗ lseg sh s u nullval
+ ⊢ lseg sh [v] x u ∗ lseg sh s u nullval.
 Proof.
 intros.
      unfold lseg at 2. Exists u. 
@@ -423,4 +422,6 @@ forward_if.
 Qed.
 
 End Proof3.
-
+(* todo they should be modules? *)
+#[export] Hint Resolve lseg_valid_pointer : valid_pointer.
+#[export] Hint Resolve lseg_local_facts : saturate_local.
